src/examples/Kuiper.Example.DotProd.fst
@@ -1,14 +1,13 @@
 module Kuiper.Example.DotProd
 
 (* Matmul dot product implemented by extracting a row and column
-   as Array1's, then computing a dot product between them. *)
+   as array1's, then computing a dot product between them. *)
 
 #lang-pulse
 
 open Kuiper
-open Kuiper.EMatrix { ematrix }
+open Kuiper.Tensor
 open Kuiper.Tensor.Layout.Alg
-module Array2 = Kuiper.Array2
 module MS = Kuiper.Spec.GEMM
 module SZ = Kuiper.SizeT
 
@@ -17,12 +16,12 @@ module SZ = Kuiper.SizeT
 i-th row of A and the j-th column of B, then computing their dot product. The
 resulting code looks just like the usual implementation."]
 fn matmul_dotprod_via_slice_f32
-  (#m #n #k : SZ.t)
-  (gA : Array2.t f32 (l2_row_major m k))
-  (gB : Array2.t f32 (l2_row_major k n))
+  (#m #n #k : sz)
+  (gA : array2 f32 (l2_row_major m k))
+  (gB : array2 f32 (l2_row_major k n))
   (i : szlt m)
   (j : szlt n)
-  (#eA #eB : ematrix f32 _ _)
+  (#eA #eB : chest2 f32 _ _)
   (#fA #fB : perm)
   preserves
     gpu ** gA |-> Frac fA eA ** gB |-> Frac fB eB
@@ -31,9 +30,9 @@ fn matmul_dotprod_via_slice_f32
   ensures
     pure (res == MS.matmul_single eA eB i j)
 {
-  // Recall some lengths
-  Array2.pts_to_ref gA;
-  Array2.pts_to_ref gB;
+  // Recall some lengths. Needed for the ctlayout instance.
+  tensor_pts_to_ref gA;
+  tensor_pts_to_ref gB;
 
   // Just call the library function that does that.
   Kuiper.DotProd.matmul_dotprod gA gB i j;
